src/Stc/CutCycles/CCTyping.v
@@ -4,6 +4,7 @@ Open Scope list_scope.
 
 From Velus Require Import Common.
 From Velus Require Import Environment.
+From Velus Require Import FunctionalEnvironment.
 From Velus Require Import Operators.
 From Velus Require Import Clocks.
 From Velus Require Import CommonProgram.
@@ -65,27 +66,28 @@ Module Type CCTYPING
 
   Section rename.
     Variable Γ Γ' : list (ident * (type * bool)).
-    Variable subl subn : Env.t ident.
+    Variable (x : var_last) (y : ident).
 
     Hypothesis Incl : forall xty,
         In xty Γ -> In xty Γ'.
-    Hypothesis SubL : forall x y ty,
-        Env.find x subl = Some y -> In (x, (ty, true)) Γ -> In (y, (ty, false)) Γ'.
-    Hypothesis SubN : forall x y ty islast,
-        Env.find x subn = Some y -> In (x, (ty, islast)) Γ -> In (y, (ty, false)) Γ'.
+    Hypothesis SubL : forall x' ty,
+        x = Last x' -> In (x', (ty, true)) Γ -> In (y, (ty, false)) Γ'.
+    Hypothesis SubN : forall x' ty islast,
+        x = Var x' -> In (x', (ty, islast)) Γ -> In (y, (ty, false)) Γ'.
 
     Lemma rename_exp_wt tys : forall e,
         wt_exp tys Γ e ->
-        wt_exp tys Γ' (rename_exp subl subn e).
+        wt_exp tys Γ' (rename_exp x y e).
     Proof.
       induction e; intros * Wt; inv Wt; simpl.
       - (* const *) constructor.
       - (* enum *) constructor; auto.
       - (* var *)
-        unfold rename_var, or_default.
-        cases_eqn Eq; econstructor; eauto.
+        unfold rename_var. cases_eqn Eq; econstructor; eauto.
+        rewrite equiv_decb_equiv in Eq0. inv Eq0. eauto.
       - (* last *)
         cases_eqn Eq; econstructor; eauto.
+        rewrite equiv_decb_equiv in Eq0. inv Eq0. eauto.
       - (* when *)
         econstructor; eauto.
       - (* unop *)
@@ -96,7 +98,7 @@ Module Type CCTYPING
 
     Lemma rename_cexp_wt tys : forall e,
         wt_cexp tys Γ e ->
-        wt_cexp tys Γ' (rename_cexp subl subn e).
+        wt_cexp tys Γ' (rename_cexp x y e).
     Proof.
       induction e using cexp_ind2'; intros * Wt; inv Wt; simpl.
       - (* merge *)
@@ -117,7 +119,7 @@ Module Type CCTYPING
 
     Lemma rename_rhs_wt tys exts : forall e,
         wt_rhs tys exts Γ e ->
-        wt_rhs tys exts Γ' (rename_rhs subl subn e).
+        wt_rhs tys exts Γ' (rename_rhs x y e).
     Proof.
       intros * Wt. inv Wt; simpl.
       - (* extcall *)
@@ -127,33 +129,38 @@ Module Type CCTYPING
     Qed.
   End rename.
 
-  Lemma rename_trconstr_wt P Γ Γ' subl subn : forall tc,
+  Lemma rename_trconstr_wt {prefs} (P: @program prefs) Γ Γ' i x y : forall tc,
       (forall xty, In xty Γ -> In xty Γ') ->
-      (forall x y ty, Env.find x subl = Some y -> In (x, (ty, true)) Γ -> In (y, (ty, false)) Γ') ->
-      (forall x y ty islast, Env.find x subn = Some y -> In (x, (ty, islast)) Γ -> In (y, (ty, false)) Γ') ->
+      (forall x' ty, x = Last x' -> In (x', (ty, true)) Γ -> In (y, (ty, false)) Γ') ->
+      (forall x' ty islast, x = Var x' -> In (x', (ty, islast)) Γ -> In (y, (ty, false)) Γ') ->
       wt_trconstr P Γ tc ->
-      wt_trconstr (cut_cycles P) Γ' (rename_trconstr subl subn tc).
+      wt_trconstr P Γ' (rename_trconstr i x y tc).
   Proof.
     intros * Incl SubL SubN Wt; inv Wt; simpl.
     - (* Def *)
-      econstructor; simpl; eauto using wt_clock_incl, rename_rhs_wt.
+      cases; econstructor; simpl; eauto using wt_clock_incl, rename_rhs_wt, wt_rhs_incl.
       + rewrite rename_rhs_typeofr; auto.
     - (* Reset State *)
       econstructor; eauto using wt_clock_incl.
     - (* Update Last *)
-      econstructor; eauto using wt_clock_incl, rename_cexp_wt.
+      cases; econstructor; eauto using wt_clock_incl, rename_cexp_wt, wt_cexp_incl.
       + rewrite rename_cexp_typeofc; auto.
     - (* Update Next *)
-      econstructor; eauto using wt_clock_incl, rename_exp_wt.
+      cases; econstructor; eauto using wt_clock_incl, rename_exp_wt, wt_exp_incl.
       + rewrite rename_exp_typeof; auto.
     - (* Reset Inst *)
       econstructor; eauto using cut_cycles_find_system, wt_clock_incl.
     - (* Update Inst *)
-      econstructor; eauto using cut_cycles_find_system; simpl_Forall;
-        eauto using wt_clock_incl, rename_exp_wt.
+      cases; econstructor; eauto; simpl_Forall;
+        eauto using wt_clock_incl, rename_exp_wt, wt_exp_incl.
       + rewrite rename_exp_typeof; auto.
-      + eapply rename_exp_wt; eauto.
-        intros * Find. rewrite Env.gempty in Find. congruence.
+  Qed.
+
+  Fact cut_cycles_wt_trconstr : forall P Γ tc,
+      wt_trconstr P Γ tc ->
+      wt_trconstr (cut_cycles P) Γ tc.
+  Proof.
+    intros * Wt; inv Wt; econstructor; eauto using cut_cycles_find_system.
   Qed.
 
   Import Fresh.
@@ -178,37 +185,49 @@ Module Type CCTYPING
         repeat constructor; simpl.
         1,3:rewrite ? map_app, ? in_app_iff.
         * left. right. left. right. solve_In.
-        * right. left. solve_In.
-        * simpl_In. simpl_Forall.
+        * right. left. simpl_In. cases. inv Hf. solve_In.
+        * simpl_In. cases. inv Hf. simpl_Forall.
           eapply wt_clock_incl; [|eauto].
           intros * In. rewrite ? map_app, ? in_app_iff in *. firstorder.
       + eapply fresh_idents_In' in H0 as In'; eauto.
         repeat constructor; simpl. 3:econstructor.
         1,3:rewrite ? map_app, ? in_app_iff.
         * left. right. left. right. solve_In.
-        * right. right. solve_In.
-        * simpl_In. simpl_Forall.
+        * right. right. simpl_In. cases. inv Hf. solve_In.
+        * simpl_In. cases. inv Hf. simpl_Forall.
           eapply wt_clock_incl; [|eauto].
           intros * In. rewrite ? map_app, ? in_app_iff in *. firstorder.
-      + eapply rename_trconstr_wt in Wt1; eauto.
-        * intros * In. rewrite ? map_app, ? in_app_iff in *. firstorder.
-        * intros * Find In.
+      + rewrite ? map_fold_rename in H1. simpl_In. simpl_Forall.
+        remember (map _ _ ++ map _ _ ++ map _ _) as Γ.
+        remember (map _ (_ ++ (_ ++ _) ++ _) ++ map _ _ ++ map _ _) as Γ'.
+        eapply fold_left_ind with (Pb:=fun '(x, lx, (_, _)) => forall ty islast, In (x, (ty, islast)) Γ' -> In (lx, (ty, false)) Γ').
+        2:eapply fold_left_ind with (Pb:=fun '(x, lx, (_, _)) => forall ty, In (x, (ty, true)) Γ' -> In (lx, (ty, false)) Γ').
+        3:eapply wt_trconstr_incl, cut_cycles_wt_trconstr; eauto.
+        * intros * Wt Incl'; destruct_conjs. eapply rename_trconstr_wt; eauto.
+          1,2:intros * Eq; inv Eq; eauto.
+        * intros * Wt Incl'; destruct_conjs. eapply rename_trconstr_wt; eauto.
+          1,2:intros * Eq; inv Eq; eauto.
+        * subst. intros * In. rewrite ? map_app, ? in_app_iff in *. firstorder.
+        * simpl_Forall. intros * In. subst.
           rewrite ? in_app_iff in In. destruct In as [In|[In|In]]; simpl_In.
           rewrite ? map_app, ? in_app_iff. left. right. left. right.
-          apply Env.from_list_find_In in Find. simpl_In. simpl_Forall.
-          eapply fresh_idents_In' in Hin0; eauto. simpl_In.
+          eapply fresh_idents_In' in H1; eauto. simpl_In. cases. inv Hf.
           eapply NoDupMembers_det in Hin; eauto using s_nodup_lasts. inv Hin.
           solve_In.
-        * intros * Find In.
+        * simpl_Forall. intros * In. subst.
           rewrite ? map_app, ? in_app_iff. left. right. left. right.
-          apply Env.from_list_find_In in Find. simpl_In. simpl_Forall.
-          eapply fresh_idents_In' in Hin; eauto. simpl_In.
-          rewrite ? in_app_iff in In. destruct In as [In|[In|In]]; simpl_In.
+          eapply fresh_idents_In' in H1; eauto. simpl_In. cases. inv Hf.
+          rewrite <-app_assoc, Permutation_app_comm with (l:=map _ (st_anns _)) in In.
+          rewrite ? app_assoc, map_app, <- ? app_assoc in In.
+          rewrite ? in_app_iff in In. destruct In as [In|[In|[In|In]]]; simpl_In.
           1:{ exfalso. eapply NoDup_app_In in ND; [|solve_In].
               eapply ND, in_app_iff, or_intror. solve_In. }
+          1:{ exfalso. eapply Facts.st_valid_AtomOrGensym_nIn; eauto using stc_not_in_lustre_prefs.
+              2:apply in_map_iff; eauto.
+              simpl. pose proof (s_good s) as (_&_&Good&_). now simpl_Forall. }
           1:{ exfalso. eapply NoDup_app_r, NoDup_app_In in ND; [|solve_In].
               eapply ND. solve_In. }
-          eapply NoDupMembers_det in Hin0; eauto using s_nodup_nexts. inv Hin0.
+          eapply NoDupMembers_det in Hin; eauto using s_nodup_nexts. inv Hin.
           solve_In.
     - intros * In.
       destruct (cut_cycles_tcs _ _ _ _) as (tcs'&st') eqn:Htcs.
@@ -218,8 +237,10 @@ Module Type CCTYPING
       firstorder.
       all:try now (eapply Wt3; rewrite ? map_app, ? in_app_iff; eauto).
       simpl_In.
-      eapply fresh_idents_In_anns2' in H0; eauto. simpl_Forall. rewrite <-map_app, filter_app in *.
-      eapply Wt3, in_app_iff. right. solve_In.
+      eapply fresh_idents_In_anns2' in H0; eauto. simpl_Forall.
+      rewrite in_app_iff in *. destruct H0; simpl_In; cases; inv Hf.
+      1,2:eapply Wt3, in_app_iff; right.
+      1,2:solve_In; eauto with datatypes; eauto.
   Qed.
 
   Lemma cut_cycles_wt_program : forall P,
